eval succeeds as well

ver2/symbolic_state_cmp.v
@@ -158,7 +158,9 @@ Definition safe_sstack_val_cmp (f_cmp : sstack_val_cmp_t) :=
     valid_bindings instk_height maxidx2 sb2 ops ->
     f_cmp sv1 sv2 maxidx1 sb1 maxidx2 sb2 instk_height ops = true ->
     forall stk mem strg ctx,
-        eval_sstack_val sv1 stk mem strg ctx maxidx1 sb1 ops = eval_sstack_val sv2 stk mem strg ctx maxidx2 sb2 ops.
+    exists v,
+      eval_sstack_val sv1 stk mem strg ctx maxidx1 sb1 ops = Some v /\
+        eval_sstack_val sv2 stk mem strg ctx maxidx2 sb2 ops = Some v.
 
 Definition safe_smemory_cmp_ext_d (smemory_cmp: smemory_cmp_ext_t) (sstack_val_cmp: sstack_val_cmp_ext_1_t) (d: nat) :=
     forall d', d' <= d -> safe_smemory_cmp (smemory_cmp (sstack_val_cmp d')).
@@ -464,7 +466,7 @@ Proof.
   intuition.
 Qed.
 
-Lemma safe_sstack_val_cmp_ext_2_d_lt:
+Lemma safe_sstack_val_cmp_ext_2_d_le:
   forall sstack_val_cmp smemory_cmp sstorage_cmp sha3_cmp d1 d2,
     d1 <= d2 -> 
     safe_sstack_val_cmp_ext_2_d sstack_val_cmp smemory_cmp sstorage_cmp sha3_cmp d2 ->
